\documentclass{article}

\usepackage[letterpaper,margin=1in]{geometry}
\usepackage{fancyhdr}
\usepackage{marginnote}
\usepackage{amsmath}
\usepackage{amssymb}
\usepackage{tikz}
\usepackage{csquotes}

\MakeOuterQuote{"}

\newcommand{\T}{\text{T}}
\newcommand{\dy}{\text{d}y}
\newcommand{\dx}{\text{d}x}
\newcommand{\e}{\text{e}}

\renewcommand{\labelitemiii}{\scriptsize$\blacksquare$}

\pagestyle{fancy}
\fancyhf{}
\rfoot{Labalme \thepage}
\rhead{(H) Linear Algebra}

\reversemarginpar

\begin{document}




\lhead{Chapter 6: Eigenvalues}
\section*{Introduction to Eigenvalues and Eigenvectors}
\begin{itemize}
    \item \marginnote{1/28:}[-8.5mm]$Ax=b=\lambda x$
    \item $Ax=\lambda x$, $\lambda\in\mathbb{F}$, $x\in\mathbb{R}^n$
    \item $\lambda$ is an eigenvalue. $\lambda x$ is an eigenvector.
    \begin{equation*}
        A=
        \begin{bmatrix}
            3 & 1\\
            1 & 3\\
        \end{bmatrix}
    \end{equation*}
    \item $
        x =
        \begin{bmatrix}
            1\\
            1\\
        \end{bmatrix}
    $ is an eigenvector of $A$ with corresponding eigenvalue of $4$.
    \item $
        \begin{bmatrix}
            3 & 1\\
            1 & 3\\
        \end{bmatrix}
        \begin{bmatrix}
            1\\
            1\\
        \end{bmatrix}
        =
        \begin{bmatrix}
            4\\
            4\\
        \end{bmatrix}
        = 4
        \begin{bmatrix}
            1\\
            1\\
        \end{bmatrix}
    $
    \begin{center}
        \begin{tikzpicture}
            \draw (-2,0) -- (2,0);
            \draw (0,-2) -- (0,2);
            \draw [thick,->] (0,0) -- node[right]{$x$} (0.5,0.5);
            \draw [thick,dashed,->] (0,0) -- node[right]{$Ax$} (2,2);
        \end{tikzpicture}
    \end{center}
    \begin{align*}
        Ax &= \lambda x\\
        Ax-\lambda x &= 0\\
        Ax-\lambda Ix &= 0\\
        (A-\lambda I)x &= 0
    \end{align*}
    \item $(A-\lambda I)x=0 \Rightarrow x\in N(A-\lambda I)^[$\footnote{To have a null space, $A-\lambda I$ has free columns.}$^] \Rightarrow |A-\lambda I|=0$
    \item $
        \begin{bmatrix}
            3 & 1\\
            1 & 3\\
        \end{bmatrix}
        -
        \begin{bmatrix}
            \lambda & 0\\
            0 & \lambda\\
        \end{bmatrix}
        =
        \begin{bmatrix}
            3-\lambda & 1\\
            1 & 3-\lambda\\
        \end{bmatrix}
    $
    \item $
        \begin{vmatrix}
            3-\lambda & 1\\
            1 & 3-\lambda\\
        \end{vmatrix}
        = 0
    $
    \begin{align*}
        0 &= (3-\lambda)^2-1^2\\
        &= 3^2-6\lambda+\lambda^2-1\\
        &= \lambda^2-6\lambda+8\\
        &= (\lambda-4)(\lambda-2)
    \end{align*}
    \item $\lambda=4,2$.
    \item $\lambda^2-6\lambda+8$ is the \textbf{characteristic polynomial} of $A$.
    \item $
        A-2I =
        \begin{bmatrix}
            -1 & 1\\
            1 & -1\\
        \end{bmatrix}
        ,\ 
        x =
        \begin{bmatrix}
            1\\
            -1\\
        \end{bmatrix}
        \in N(A-2I)
    $.
    \item $
        A-4I =
        \begin{bmatrix}
            -1 & 1\\
            1 & -1\\
        \end{bmatrix}
        ,\ 
        x =
        \begin{bmatrix}
            1\\
            1\\
        \end{bmatrix}
        \in N(A-4I)
    $.
    \item "Eigenspace" is not $\mathbb{R}^2$, but two lines in $\mathbb{R}^2$, specifically $y=\pm x$.
    \begin{itemize}
        \item $y=\pm x$ comes from $c_1\begin{bmatrix}1\\1\end{bmatrix}$ and $c_2\begin{bmatrix}1\\-1\end{bmatrix}$.
    \end{itemize}

    %%%%%%%%%%%%%%%%%%%%%%

    \marginnote{1/29:}\begin{equation*}
        A =
        \begin{bmatrix}
            2 & -2 & 3\\
            0 & 3 & -2\\
            0 & -1 & 2\\
        \end{bmatrix}
    \end{equation*}
    \begin{align*}
        P(\lambda) &= |A-\lambda I|\\
        &=
        \begin{vmatrix}
            2-\lambda & -2 & 3\\
            0 & 3-\lambda & -2\\
            0 & -1 & 2-\lambda\\
        \end{vmatrix}\\
        &= -1
        \begin{vmatrix}
            2-\lambda & 3\\
            0 & -2\\
        \end{vmatrix}
        (-1)^{3+2} + (2-\lambda)
        \begin{vmatrix}
            2-\lambda & -2\\
            0 & 3-\lambda\\
        \end{vmatrix}
        (-1)^{3+3}\\
        &= ((2-\lambda)(-2))+(2-\lambda)((2-\lambda)(3-\lambda))\\
        &= -4+2\lambda+(2-\lambda)^2(3-\lambda)\\
        &= -4+2\lambda+(4-4\lambda+\lambda^2)(3-\lambda)\\
        &= -4+2\lambda+12-4\lambda-12\lambda+4\lambda^2+3\lambda^2-\lambda^3\\
        &= -\lambda^3+7\lambda^2-14\lambda+8\\
        &= -(\lambda-1)(\lambda-2)(\lambda-4)
    \end{align*}
    \begin{align*}
        A-I &=
        \begin{bmatrix}
            1 & -2 & 3\\
            0 & 2 & -2\\
            0 & -1 & 1\\
        \end{bmatrix}&
        A-2I &=
        \begin{bmatrix}
            0 & -2 & 3\\
            0 & 1 & -2\\
            0 & -1 & 0\\
        \end{bmatrix}&
        A-4I &=
        \begin{bmatrix}
            -2 & -2 & 3\\
            0 & -1 & -2\\
            0 & -1 & -2\\
        \end{bmatrix}&
    \end{align*}
    \item $P(\lambda)$ is positive when $n\in 2\mathbb{N}$, negative otherwise.
    \begin{itemize}
        \item Signs flip term to term (think about binomial expansion).
    \end{itemize}
    \item Coefficients of the $n-1$ degree term is the sum of the diagonal entries.
    \item Coefficient of the $0^\text{th}$ degree term is $|A|$.
    \begin{itemize}
        \item $P_\lambda(0) = |A-0\cdot I| = |A|$.
    \end{itemize}
    \item Product of the eigenvalues is $|A|$.
    \begin{itemize}
        \item Think about expanding the factorization.
    \end{itemize}
    \item Eigenvalues of $U$ are the diagonal values.
    \begin{itemize}
        \item $\lambda_1\lambda_2\cdots\lambda_n=|A|$, which is the product of the diagonal entries.
        \item $\lambda_1+\cdots+\lambda_n=\text{trace}(A)$, which is the sum of the diagonal entries.
    \end{itemize}
    \item $Ax=\lambda x$
    \begin{itemize}
        \item $A^2x=AAx=A\lambda x=\lambda Ax=\lambda\lambda x=\lambda^2x$
    \end{itemize}
\end{itemize}



\section*{Similarity}
\begin{itemize}
    \item \marginnote{1/30:}$A\sim B$$^[$\footnote{$A$ "is similar to" $B$}$^]$ iff $\exists\ S:A=SBS^{-1},\ B=S^{-1}AS$.
    \begin{enumerate}
        \item If $A\sim B$, then $|A|=|B|$.
        \begin{align*}
            B &= S^{-1}AS\\
            |B| &= |S^{-1}AS|\\
            |B| &= |S^{-1}||A||S|\\
            |B| &= \frac{1}{|S|}|A||S|\\
            |B| &= |A|
        \end{align*}
        \item If $A\sim B$, then they share the same characteristic polynomial.
        \begin{align*}
            B &= S^{-1}AS\\
            |B-\lambda I| &= |S^{-1}AS-\lambda I|\\
            &= |S^{-1}AS-\lambda S^{-1}IS|\\
            &= |S^{-1}S(A-\lambda I)|\\
            &= |I(A-\lambda I)|\\
            |B-\lambda I| &= |A-\lambda I|
        \end{align*}
        \begin{itemize}
            \item If they have the same characteristic polynomial, $\therefore$ $A$ and $B$ have the same eigenvalues.
        \end{itemize}
    \end{enumerate}
    \item What is the best possible $B$ if $A\sim B$?
    \begin{itemize}
        \item Sparse.
        \item Diagonal.
        \item $
            A=[\text{ugly}]\quad\rightarrow\quad
            B=\begin{bmatrix}
                \lambda_1 &  & 0\\
                 & \ddots & \\
                0 &  & \lambda_n\\
            \end{bmatrix}
            =\Lambda
        $
    \end{itemize}
    \item \textbf{Diagonalization}:
    \begin{align*}
        A &= S\Lambda S^{-1}\\
        AS &= S\Lambda\\
        \Lambda &= S^{-1}AS
    \end{align*}
    \item $A=S\Lambda S^{-1}$
    \begin{itemize}
        \item $A^2 = AA = S\Lambda S^{-1}S\Lambda S^{-1} = S\Lambda\Lambda S^{-1} = S\Lambda^2 S^{-1}$
        \item $A^k = S\Lambda^k S^{-1}$
        \item $
            A^k = S
            \begin{bmatrix}
                {\lambda_1}^k &  & 0\\
                 & \ddots & \\
                0 &  & {\lambda_n}^k\\
            \end{bmatrix}
            S^{-1}
        $
    \end{itemize}
    \item Diagonalize the following matrix $A$.
    \begin{equation*}
        A =
        \begin{bmatrix}
            -1 & 0 & 1\\
            3 & 0 & -3\\
            1 & 0 & -1\\
        \end{bmatrix}
    \end{equation*}
    \begin{itemize}
        \item Find the characteristic polynomial.
        \begin{align*}
            |A-\lambda I| &=
            \begin{vmatrix}
                -1-\lambda & 0 & 1\\
                3 & 0-\lambda & -3\\
                1 & 0 & -1-\lambda\\
            \end{vmatrix}\\
            &= (-1-\lambda)((-\lambda)(-1-\lambda))+(-1)(-\lambda)\\
            &= -\lambda(-1-\lambda)^2+\lambda\\
            &= -\lambda(1+2\lambda+\lambda^2)+\lambda\\
            &= -\lambda^3-2\lambda^2\\
            &= -\lambda^2(\lambda+2)
        \end{align*}
        \item Find the eigenvalues: $\lambda_1=\lambda_2=0$, $\lambda_3=-2$
        \item \textbf{Algebraic multiplicity} of $\lambda_1,\lambda_2$ is 2.
        \item A.M. of $\lambda_3$ is 1.
        \item $
            A-0I =
            \begin{bmatrix}
                -1 & 0 & 1\\
                3 & 0 & -3\\
                1 & 0 & -1\\
            \end{bmatrix}
        $
        \item $\text{rank}(A-0I)=1 \Rightarrow \dim(N(A-0I))=2$
        \item The 2 directly above is the \textbf{geometric multiplicity}.
        \item $A$ is diagonalizable iff A.M. of $\lambda_i=\text{G.M.}$
        
        %%%%%%%%%%%%%%%%%%%%%%%%%
        
        \item \marginnote{1/31:}Eigenvectors are $
            x_1=
            \begin{bmatrix}
                1\\
                0\\
                1\\
            \end{bmatrix}
        $ and $
            x_2=
            \begin{bmatrix}
                0\\
                1\\
                0\\
            \end{bmatrix}
        $.
        \item $
        A+2I =
        \begin{bmatrix}
            1 & 0 & 1\\
            3 & 2 & -3\\
            1 & 0 & 1\\
        \end{bmatrix}
    $
        \item Eigenvector is $
            x_3=
            \begin{bmatrix}
                1\\
                -3\\
                -1\\
            \end{bmatrix}
        $
        \item Use an $S$ matrix of eigenvectors.
        \item $
            A = S\Lambda S^{-1} = \frac{1}{2}
            \begin{bmatrix}
                0 & 1 & 1\\
                1 & 0 & -3\\
                0 & 1 & -1\\
            \end{bmatrix}
            \begin{bmatrix}
                0 &  & \\
                 & 0 & \\
                 &  & -2\\
            \end{bmatrix}
            \begin{bmatrix}
                3 & 2 & -3\\
                1 & 0 & 1\\
                1 & 0 & -1\\
            \end{bmatrix}
        $
        \item Note that $
            A^{9752} = \frac{1}{2}
            \begin{bmatrix}
                0 & 1 & 1\\
                1 & 0 & -3\\
                0 & 1 & -1\\
            \end{bmatrix}
            \begin{bmatrix}
                0 &  & \\
                 & 0 & \\
                 &  & (-2)^{9752}\\
            \end{bmatrix}
            \begin{bmatrix}
                3 & 2 & -3\\
                1 & 0 & 1\\
                1 & 0 & -1\\
            \end{bmatrix}
        $
    \end{itemize}
    \item \textbf{Algebraic multiplicity}: The number of repeated roots to a polynomial. For all of the roots, it adds up to $n$ ($n$-square matrix). \emph{Also known as} \textbf{A.M.}
    \item \textbf{Geometric multiplicity}: The number of eigenvectors produced from each root. For all of the roots, it may not add up to $n$ ($n$-square matrix). $\dim(N(A-\lambda I))$. \emph{Also known as} \textbf{G.M.}
    \item A nondiagonalizable example:
    \begin{equation*}
        A =
        \begin{bmatrix}
            1 & 1 & 0\\
            0 & 1 & 1\\
            0 & 0 & 4\\
        \end{bmatrix}
    \end{equation*}
    \begin{itemize}
        \item $\lambda_1 = \lambda_2 = 1$ and $\lambda_3 = 4$.
        \item $\lambda_1$ and $\lambda_2$ have $\text{A.M.}={\color{red}2}$.
        \item $\lambda_3$ has $\text{A.M.}=1$.
        \item $
            A-I=
            \begin{bmatrix}
                0 & 1 & 0\\
                0 & 0 & 1\\
                0 & 0 & 3\\
            \end{bmatrix}
        $
        \item $\text{rank}(A-I)=2\Rightarrow\dim(N(A-I))=1\Rightarrow\text{G.M.}={\color{red}1}$.
        \item $
            x_1=
            \begin{bmatrix}
                1\\
                0\\
                0\\
            \end{bmatrix}
        $
        \item $
            A-4I=
            \begin{bmatrix}
                -3 & 1 & 0\\
                0 & -3 & 1\\
                0 & 0 & 0\\
            \end{bmatrix}
        $
        \item $
            x_2=
            \begin{bmatrix}
                1\\
                3\\
                9\\
            \end{bmatrix}
        $
        \item $S$ would be $3\times 2$ and, thus, not square, so $\nexists\ S^{-1}$$^[$\footnote{At a later date, we will look at an analogy of projections to diagonalization that finds the "best possible" diagonalization (which may not be perfectly diagonal).}$^]$.
    \end{itemize}
    \item \textbf{Canonical} (form): An accepted way of expressing something.
\end{itemize}



\section*{Markov Chains}
\marginnote{2/3:}
\begin{center}
    \begin{tikzpicture}
        \node (pgh) [circle,draw] {PGH};
        \node (cle) [circle,draw] at (5,0) {CLE};
        \draw [->,thick] (pgh.30) to[bend left=30] node[above]{0.05} (cle.150);
        \draw [->,thick] (cle.-150) to[bend left=30] node[below]{0.2} (pgh.-30);
        \draw [->,thick] (pgh.90) to[bend right=100,looseness=3] node[above]{0.95} (pgh.150);
        \draw [->,thick] (cle.90) to[bend left=100,looseness=3] node[above]{0.8} (cle.30);
    \end{tikzpicture}
\end{center}
\begin{itemize}
    \item $
        u_0 =
        \begin{bmatrix}
            500,000\\
            500,000\\
        \end{bmatrix}
    $
    \item $Au_0 = u_1$.
    \item $Au_1 = u_2$, $A(Au_0) = u_2$, $A^2u_0 = u_2$, $A^ku_0 = u_k$, $(S\Lambda S^{-1})^ku_0 = u_k$, $S\Lambda^kS^{-1}u_0 = u_k$.
    \begin{align*}
        A &=
        \begin{bmatrix}
            0.95 & 0.20\\
            0.05 & 0.80\\
        \end{bmatrix}&
        u_k &=
        \begin{bmatrix}
            \text{PGH}\\
            \text{CLE}\\
        \end{bmatrix}
    \end{align*}
    \item $A$ is a \textbf{Markov matrix}, where all columns and rows add to 1.
    \item $
        Au_0 =
        \begin{bmatrix}
            0.95 & 0.20\\
            0.05 & 0.80\\
        \end{bmatrix}
        \begin{bmatrix}
            500,000\\
            500,000\\
        \end{bmatrix}
        = u_1
    $
    \begin{align*}
        |A-\lambda I| &=
        \begin{vmatrix}
            0.95-\lambda & 0.20\\
            0.05 & 0.80-\lambda\\
        \end{vmatrix}\\
        &= (0.95-\lambda)(0.8-\lambda)-(0.2)(0.05)\\
        &= (\lambda-1)(\lambda-0.75)
    \end{align*}
    \item $\lambda_1 = 1,\ \lambda_2 = 0.75$.
    \item $
        A-I =
        \begin{bmatrix}
            -0.05 & 0.2\\
            0.05 & -0.2\\
        \end{bmatrix}
        \Rightarrow
        x =
        \begin{bmatrix}
            4\\
            1\\
        \end{bmatrix}
    $
    \item $
        A-0.75I =
        \begin{bmatrix}
            0.2 & 0.2\\
            0.05 & 0.05\\
        \end{bmatrix}
        \Rightarrow
        x =
        \begin{bmatrix}
            -1\\
            1\\
        \end{bmatrix}
    $
    \begin{align*}
        A^ku_0 &= \frac{1}{5}
        \begin{bmatrix}
            4 & -1\\
            1 & 1\\
        \end{bmatrix}
        \begin{bmatrix}
            1 & 0\\
            0 & 0.75\\
        \end{bmatrix}^k
        \begin{bmatrix}
            1 & 1\\
            -1 & 4\\
        \end{bmatrix}
        \begin{bmatrix}
            500,000\\
            500,000\\
        \end{bmatrix}\\
        &=
        \begin{bmatrix}
            4 & -1\\
            1 & 1\\
        \end{bmatrix}
        \begin{bmatrix}
            1 & 0\\
            0 & 0.75^k\\
        \end{bmatrix}
        \begin{bmatrix}
            200,000\\
            300,000\\
        \end{bmatrix}\\
        &=
        \begin{bmatrix}
            4\\
            1\\
        \end{bmatrix}
        (200,000) +
        \begin{bmatrix}
            -1\\
            1\\
        \end{bmatrix}
        (0.75)^k(300,000)
    \end{align*}
    \item $
        \begin{bmatrix}
            800,000\\
            200,000\\
        \end{bmatrix}
    $ is the steady-state vector.
    \item $
        \begin{bmatrix}
            -(0.75)^k(300,000)\\
            (0.75)^k(300,000)\\
        \end{bmatrix}
    $ is the dynamically changing vector.
    \item $
        \lim_{k\to\infty} A^ku_0 =
        \begin{bmatrix}
            800,000\\
            200,000\\
        \end{bmatrix}
        =
        \begin{bmatrix}
            \text{PGH}\\
            \text{CLE}\\
        \end{bmatrix}
    $
\end{itemize}


\subsection*{Explicit Formula for the Fibonacci Sequence}
\begin{itemize}
    \item \marginnote{2/4:}1, 1, 2, 3, 5, 8, \dots
    \item Recursively defined formula: $F_n$$^[$\footnote{The $n$-th Fibonacci number.}$^]$$=F_{n-1}+F_{n-2}$.
    \begin{align*}
        F_n &= F_{n-1}+F_{n-2}\\
        F_{n-1} &= F_{n-1}\\
        \begin{bmatrix}
            F_n\\
            F_{n-1}\\
        \end{bmatrix}
        &=
        \begin{bmatrix}
            1 & 1\\
            1 & 0\\
        \end{bmatrix}
        \begin{bmatrix}
            F_{n-1}\\
            F_{n-2}\\
        \end{bmatrix}
    \end{align*}
    \item $u_n = A^nu_0 = S\Lambda^nS^{-1}u_0$.
    \begin{align*}
        0 &= |A-\lambda I|\\
        &=
        \begin{vmatrix}
            1-\lambda & 1\\
            1 & -\lambda\\
        \end{vmatrix}\\
        &= -\lambda(1-\lambda)-1\\
        &= \lambda^2-\lambda-1
    \end{align*}
    \item $\lambda = \frac{1\pm\sqrt{5}}{2}$$^[$\footnote{This is the Golden ratio!}$^]$.
    \item $\lambda_1 = \frac{1+\sqrt{5}}{2}$.
    \begin{align*}
        N(A-\lambda_1I) &= N\left(
        \begin{bmatrix}
            1-\frac{1+\sqrt{5}}{2} & 1\\
            1 & -\frac{1+\sqrt{5}}{2}\\
        \end{bmatrix}
        \right)\\
        &= N\left(
        \begin{bmatrix}
            \frac{1-\sqrt{5}}{2} & 1\\
            1 & \frac{-1-\sqrt{5}}{2}\\
        \end{bmatrix}
        \right)\\
    \end{align*}
    \item $
        \begin{bmatrix}
            \frac{1-\sqrt{5}}{2} & 1\\
            1 & \frac{-1-\sqrt{5}}{2}\\
        \end{bmatrix}
        \begin{bmatrix}
            x_1\\
            x_2\\
        \end{bmatrix}
        =
        \begin{bmatrix}
            0\\
            0\\
        \end{bmatrix}
    $
    \item Let $x_2=1$.
    \begin{align*}
        \frac{1-\sqrt{5}}{2}x_1+1 &= 0\\
        \frac{1-\sqrt{5}}{2}x_1 &= -\frac{2}{2}\\
        x_1 &= \frac{-2}{1-\sqrt{5}}\times \frac{1+\sqrt{5}}{1+\sqrt{5}}\\
        &= \frac{-2-2\sqrt{5}}{-4}\\
        &= \frac{1+\sqrt{5}}{2}
    \end{align*}
    \item $
        s_1 =
        \begin{bmatrix}
            \frac{1+\sqrt{5}}{2}\\
            1\\
        \end{bmatrix}
    $, $
        s_2 =
        \begin{bmatrix}
            \frac{1-\sqrt{5}}{2}\\
            1\\
        \end{bmatrix}
    $.
    \item $
        \begin{bmatrix}
            1 & 1\\
            1 & 0\\
        \end{bmatrix}
        =
        \begin{bmatrix}
            \frac{1+\sqrt{5}}{2} & \frac{1-\sqrt{5}}{2}\\
            1 & 1\\
        \end{bmatrix}
        \begin{bmatrix}
            \frac{1+\sqrt{5}}{2} & 0\\
            0 & \frac{1-\sqrt{5}}{2}\\
        \end{bmatrix}
        S^{-1}
    $
    \item $
        S^{-1}
        = \frac{1}{|S|}C_S^\T
        = \frac{1}{\sqrt{5}}
        \begin{bmatrix}
            1 & \frac{-1+\sqrt{5}}{2}\\
            -1 & \frac{1+\sqrt{5}}{2}\\
        \end{bmatrix}
    $
    \item $u_k = A^ku_0 = S\Lambda^kS^{-1}u_0$.
    \begin{align*}
        S^{-1}u_0 &= \frac{1}{\sqrt{5}}
        \begin{bmatrix}
            1 & \frac{-1+\sqrt{5}}{2}\\
            -1 & \frac{1+\sqrt{5}}{2}\\
        \end{bmatrix}
        \begin{bmatrix}
            1\\
            1\\
        \end{bmatrix}\\
        &= \frac{1}{\sqrt{5}}
        \begin{bmatrix}
            \frac{1+\sqrt{5}}{2}\\
            \frac{-1+\sqrt{5}}{2}\\
        \end{bmatrix}\\
        &=
        \begin{bmatrix}
            \frac{1+\sqrt{5}}{2\sqrt{5}}\\
            \frac{-1+\sqrt{5}}{2\sqrt{5}}\\
        \end{bmatrix}\\
        &=
        \begin{bmatrix}
            \frac{5+\sqrt{5}}{10}\\
            \frac{5-\sqrt{5}}{10}\\
        \end{bmatrix}
    \end{align*}
    \item $
        u_k =
        \begin{bmatrix}
            \frac{1+\sqrt{5}}{2}\\
            1\\
        \end{bmatrix}
        \left( \frac{1+\sqrt{5}}{2} \right)^k\left( \frac{5+\sqrt{5}}{10} \right)+
        \begin{bmatrix}
            \frac{1-\sqrt{5}}{2}\\
            1\\
        \end{bmatrix}
        \left( \frac{1-\sqrt{5}}{2} \right)^k\left( \frac{5-\sqrt{5}}{10} \right)
    $
\end{itemize}



\section*{Systems of First-Order Ordinary Differential Equations}
\begin{itemize}
    \item \marginnote{2/11:}Let $f(x)=y$ and $a,c,K\in\mathbb{F}$.
    \begin{align*}
        \frac{\dy}{\dx} &= ay\\
        \frac{1}{y}\frac{\dy}{\dx} &= a\\
        \frac{1}{y}\frac{\dy}{\dx}\, \dx &= a\, \dx\\
        \frac{1}{y}\, \dy &= a\, \dx\\
        \int \frac{1}{y}\, \dy &= \int a\, \dx\\
        \ln y &= ax+c\\
        y &= \e^{ax+c}\\
        &= \e^{ax}\text{e}^c\\
        &= K\e^{ax}
    \end{align*}
    \item Let $\frac{\dy}{\dx}=y'$.
    \begin{itemize}
        \item $y_1' = a_{11}y_1+a_{12}y_2+\cdots+a_{1n}y_n$.
        \item $y_2' = a_{21}y_1+a_{22}y_2+\cdots+a_{2n}y_n$.
        \item $\vdots$
        \item $y_n' = a_{n1}y_1+a_{n2}y_2+\cdots+a_{nn}y_n$.
    \end{itemize}
    \item This is a \textbf{square system} of equations.
    \item Rewrite as $y' = Ay$.
    \begin{equation*}
        \begin{bmatrix}
            y_1'\\
            y_2'\\
            \vdots\\
            y_n'\\
        \end{bmatrix}
        =
        \begin{bmatrix}
            a_{11} & a_{12} & \cdots & a_{1n}\\
            a_{21} & a_{22} & \cdots & a_{2n}\\
            \vdots &        & \ddots &       \\
            a_{n1} & a_{n2} & \cdots & a_{nn}\\
        \end{bmatrix}
        \begin{bmatrix}
            y_1\\
            y_2\\
            \vdots\\
            y_n\\
        \end{bmatrix}
    \end{equation*}
    \item Solve the following system of differential equations.
    \begin{align*}
        y_1' &= 3y_1\\
        y_2' &= -2y_2\\
        y_3' &= 5y_3
    \end{align*}
    \begin{equation*}
        \begin{bmatrix}
            y_1'\\
            y_2'\\
            y_3'\\
        \end{bmatrix}
        =
        \begin{bmatrix}
            3 & 0 & 0\\
            0 & -2 & 0\\
            0 & 0 & 5\\
        \end{bmatrix}
        \begin{bmatrix}
            y_1\\
            y_2\\
            y_3\\
        \end{bmatrix}
    \end{equation*}
    \begin{itemize}
        \item General Solution:
    \end{itemize}
    \begin{align*}
        y_1 &= k_1\e^{3x}\\
        y_2 &= k_2\e^{-2x}\\
        y_3 &= k_3\e^{5x}
    \end{align*}
    \begin{itemize}
        \item Particular Solution (where $y_1(0)=2$, $y_2(0)=-1$, and $y_3(0)=7$ are the initial conditions):
    \end{itemize}
    \begin{align*}
        y_1 &= 2\e^{3x}\\
        y_2 &= -\e^{-2x}\\
        y_3 &= 7\e^{5x}
    \end{align*}
    \item Consider a different system. Remember throughout that we are solving for $y$.
    \begin{align*}
        y_1' &= y_1+y_2\\
        y_2' &= 4y_1-2y_2
    \end{align*}
    \begin{itemize}
        \item The previous system was so easy to solve because the matrix was diagonal. This one (as follows) will not be. Therefore, we should diagonalize it.
    \end{itemize}
    \begin{equation*}
        \begin{bmatrix}
            y_1'\\
            y_2'\\
        \end{bmatrix}
        =
        \begin{bmatrix}
            1 & 1\\
            4 & -2\\
        \end{bmatrix}
        \begin{bmatrix}
            y_1\\
            y_2\\
        \end{bmatrix}
    \end{equation*}
    \begin{itemize}
        \item Start with $y'=Ay$.
        \item Substitute $y=Su$.
        \begin{itemize}
            \item Note that $y=Su\Rightarrow y'=Su'$$^[$\footnote{Think about differentiating both sides: $y\rightarrow y'$ is obvious, $S$ will be unchanged because it's just coefficients, and the functions of $u$ will be differentiated.}$^]$.
            \item If we can find $u'$ in terms of a diagonal matrix and $u$, we can solve for $y$.
        \end{itemize}
        \begin{center}
            \begin{tikzpicture}
                \draw (-2,0) -- (2,0) node[right]{
                    $
                        \begin{bmatrix}
                            1\\
                            0\\
                        \end{bmatrix}
                    $
                };
                \draw (0,-2) -- (0,2) node[above]{
                    $
                        \begin{bmatrix}
                            0\\
                            1\\
                        \end{bmatrix}
                    $
                };

                \draw [dashed] (-0.5,2) node[above]{$S_2$} -- (0.5,-2);
                \draw [dashed] (-2,-0.7) -- (2,0.7) node[right]{$S_1$};

                \draw [red,thick] (-1,2) to[out=-45,in=180] (1.8,1.3);
                \draw [red,thick] plot[smooth,tension=1.2] coordinates{
                    (-1,-1) (-0.5,-0.3) (0.2,-0.6) (1,0.4)
                };
            \end{tikzpicture}
        \end{center}
        \item We seek to find a new basis $S$ such that the matrix scaling $u$ will be diagonal.
    \end{itemize}
    \begin{align*}
        Su' &= Ay\\
        Su' &= ASu\\
        u' &= S^{-1}ASu\\
        u' &= \Lambda u
    \end{align*}
    \begin{itemize}
        \item The last substitution above is legal because if $A=S\Lambda S^{-1}$, then $\Lambda=S^{-1}AS$.
    \end{itemize}
    \begin{align*}
        0 &=
        \begin{vmatrix}
            1-\lambda & 1\\
            4 & -2-\lambda\\
        \end{vmatrix}\\
        &= (1-\lambda)(-2-\lambda)-4\\
        &= -2-\lambda+2\lambda+\lambda^2-4\\
        &= \lambda^2+\lambda-6\\
        &= (\lambda-2)(\lambda+3)
    \end{align*}
    \begin{align*}
        \lambda_1 &= 2&
        \lambda_2 &= -3
    \end{align*}
    \begin{itemize}
        \item $
            A-2I=
            \begin{bmatrix}
                -1 & 1\\
                4 & -4\\
            \end{bmatrix}
            \begin{bmatrix}
                1\\
                1\\
            \end{bmatrix}
            =
            \begin{bmatrix}
                0\\
                0\\
            \end{bmatrix}
        $
        \item $
            A+3I=
            \begin{bmatrix}
                4 & 1\\
                4 & 1\\
            \end{bmatrix}
            \begin{bmatrix}
                -1\\
                4\\
            \end{bmatrix}
            =
            \begin{bmatrix}
                0\\
                0\\
            \end{bmatrix}
        $
    \end{itemize}
    \begin{align*}
        u' &= \Lambda u\\
        \begin{bmatrix}
            u_1'\\
            u_2'\\
        \end{bmatrix}
        &=
        \begin{bmatrix}
            2 & 0\\
            0 & -3\\
        \end{bmatrix}
        \begin{bmatrix}
            u_1\\
            u_2\\
        \end{bmatrix}
    \end{align*}
    \begin{align*}
        u_1 &= k_1\e^{2x}\\
        u_2 &= k_2\e^{-3x}
    \end{align*}
    \begin{align*}
        y &= Su\\
        \begin{bmatrix}
            y_1\\
            y_2\\
        \end{bmatrix}
        &=
        \begin{bmatrix}
            1 & -1\\
            1 & 4\\
        \end{bmatrix}
        \begin{bmatrix}
            k_1\e^{2x}\\
            k_2\e^{-3x}\\
        \end{bmatrix}
    \end{align*}
    \begin{align*}
        y_1 &= k_1\e^{2x}-k_2\e^{-3x}\\
        y_2 &= k_1\e^{2x}+4k_2\e^{-3x}
    \end{align*}
\end{itemize}




\end{document}